SkLean/Ast2.lean
@@ -1,0 +1,243 @@
+import Mathlib.Tactic
+
+mutual
+
+inductive M where
+  | mk :  ℕ → M
+deriving Repr
+
+inductive S where
+  | mk : ℕ → S
+deriving DecidableEq, Repr, BEq
+
+inductive K where
+  | mk : ℕ → K
+deriving DecidableEq, Repr, BEq
+
+inductive Call where
+  | mk : Expr → Expr → Call
+deriving DecidableEq, Repr, BEq
+
+inductive Expr where
+  | m    : M → Expr
+  | k    : K → Expr
+  | s    : S → Expr
+  | call : Call → Expr
+deriving DecidableEq, Repr, BEq
+
+end
+
+namespace Call
+
+def lhs : Call → Expr
+  | .mk lhs _ => lhs
+
+def rhs : Call → Expr
+  | .mk _ rhs => rhs
+
+end Call
+
+/-
+## DSL
+
+We make use of a small DSL for legibility.
+-/
+
+declare_syntax_cat skmexpr
+syntax "K" ident               : skmexpr
+syntax "S" ident               : skmexpr
+syntax "M" ident               : skmexpr
+syntax "K" num                 : skmexpr
+syntax "S" num                 : skmexpr
+syntax "M" num                 : skmexpr
+syntax "(" skmexpr skmexpr ")" : skmexpr
+syntax ident                   : skmexpr
+syntax "(" skmexpr ")"         : skmexpr
+
+syntax " ⟪ " skmexpr " ⟫ "     : term
+
+macro_rules
+  | `(⟪ K $u:ident ⟫)                     => `(Expr.k (.mk $u))
+  | `(⟪ S $u:ident ⟫)                     => `(Expr.s (.mk $u))
+  | `(⟪ M $u:ident ⟫)                     => `(Expr.m (.mk $u))
+  | `(⟪ K $u:num ⟫)                       => `(Expr.k (.mk $u))
+  | `(⟪ S $u:num ⟫)                       => `(Expr.s (.mk $u))
+  | `(⟪ M $u:num ⟫)                       => `(Expr.m (.mk $u))
+  | `(⟪ $e:ident ⟫)                       => `($e)
+  | `(⟪ ($e:skmexpr) ⟫)                   => `(⟪$e⟫)
+  | `(⟪ ($e₁:skmexpr $e₂:skmexpr) ⟫)      => `(Expr.call (.mk ⟪ $e₁ ⟫ ⟪ $e₂ ⟫))
+
+syntax "SKM[ " skmexpr " ] "        : term
+syntax "SKC[" skmexpr skmexpr "]" : term
+
+macro_rules
+  | `(SKM[ $e:skmexpr ]) => `(⟪ $e ⟫)
+
+macro_rules
+  | `(SKC[ $e₁:skmexpr $e₂:skmexpr ]) => `(Call.mk ⟪ $e₁ ⟫ ⟪ $e₂ ⟫)
+
+namespace Expr
+
+def max_universe (e : Expr) : ℕ :=
+  match e with
+    | SKM[(K n)] => n
+    | SKM[(S n)] => n
+    | SKM[(M n)] => n
+    | SKM[(lhs rhs)] =>
+      (max_universe lhs) + (max_universe rhs)
+
+def min_universe (e : Expr) : ℕ :=
+  match e with
+    | SKM[(K n)] => n
+    | SKM[(S n)] => n
+    | SKM[(M n)] => n
+    | SKM[(lhs rhs)] =>
+      min (max_universe lhs) (max_universe rhs)
+
+inductive valid_universes : Expr → Prop
+  | k    : valid_universes SKM[(K n)]
+  | s    : valid_universes SKM[(S n)]
+  | m    : valid_universes SKM[(M n)]
+  | call : lhs.max_universe > rhs.max_universe
+    → valid_universes lhs
+    → valid_universes rhs
+    → valid_universes SKM[(lhs rhs)]
+
+end Expr
+
+/-
+## Judgment Rules
+
+`K`, `M`, and `S` must be well-typed on their own. We need some expression that can represent the type of `K`. One option is the \\(\rightarrow\\) type constructor from the SLTC or System F. The typing of \\(S\\) and \\(K\\) are fairly obvious. However, the typing of \\(M\\) is not. It's not immediately clear that we need typing judgment rules for `K`, `M`, or `S` alone. There is no way to explicitly assign a type to `K`, `M`, or `S`. They just are. However, there are emergent rules for application. The typical rules for application in the SK combinator calculus are as follows:
+
+$$
+K : \alpha \rightarrow \beta \rightarrow \alpha \\\\
+S : (\alpha \rightarrow \beta \rightarrow \gamma) \rightarrow (\alpha \rightarrow \beta) \rightarrow \alpha \rightarrow \gamma \\\\
+M : hmm
+$$
+
+Typing rules quickly beome complicated. We would prefer to avoid binders in our type discipline. We can create an "emergent" typing based on function application.
+
+$$
+\frac{
+  \Gamma \vdash e_{1} : T
+}{
+  \Gamma \vdash K\ e_{1}\ e_{2} : T
+}
+$$
+$$
+\frac{
+  \Gamma \vdash f_{1}\ \text{arg}\ (f_{2}\ \text{arg}) : T)
+}{
+  \Gamma \vdash S\ f_{1}\ f_{2}\ \text{arg} : T
+}
+$$
+
+But what is the type of \\(K\\)? It's not really obvious. Clearly, we need some way to represent the type of \\(K\\) that avoids binders. Recall that:
+
+$$
+Kxy = x
+$$
+
+The type of \\(K\\) is typically \\(\alpha \rightarrow \beta \rightarrow \alpha\\). Its type is of the form of the \\(K\\) combinator. We can thus define a typing as such:
+
+$$
+K : K
+$$
+
+This typing is coherent under an evaluation rule for the \\(M\\) combinator:
+
+$$
+M\ (x : t)\ \text{arg} = \text{arg}\ x\ (\text{arg}\ t) \\\\
+M\ \mathbb{N}\ K = K\ \mathbb{N}\ (K\ \text{Type}) = \mathbb{N} \\\\
+M\ K\ K = K\ K\ (K\ K) = K
+$$
+-/
+
+mutual
+inductive is_eval_once : Expr → Expr → Prop
+  | k x y n      : is_eval_once SKM[((K n x) y)] x
+  | s x y z n    : is_eval_once SKM[(((S n x) y) z)] SKM[((x z) (y z))]
+  | m e t n      : valid_judgment e t
+    → is_eval_once SKM[((M n) e)] t
+  | left         : is_eval_once lhs lhs'
+    → is_eval_once SKM[(lhs rhs)] SKM[(lhs' rhs)]
+
+inductive is_eval_once_weak : Expr → Expr → Prop
+  | k x y n      : is_eval_once_weak SKM[((K n x) y)] x
+  | s x y z n    : is_eval_once_weak SKM[(((S n x) y) z)] SKM[((x z) (y z))]
+  | m e t n      : valid_judgment_weak e t
+    → is_eval_once_weak SKM[((M n) e)] t
+  | left         : is_eval_once_weak lhs lhs'
+    → is_eval_once_weak SKM[(lhs rhs)] SKM[(lhs' rhs)]
+
+inductive beta_eq : SkExpr → SkExpr → Prop
+  | rfl                       : beta_eq e e
+  | eval                      : is_eval_once e₁ e₂ → beta_eq e₁ e₂
+  | left                      : beta_eq lhs lhs'   → beta_eq SKM[(lhs rhs)] SKM[(lhs' rhs)]
+  | trans                     : beta_eq e₁ e₂ → beta_eq e₂ e₃ → beta_eq e₁ e₃
+
+inductive valid_judgment : Expr → Expr → Prop
+  | k n                       : valid_judgment SKM[K n] (.k (.mk n.succ))
+  | s n                       : valid_judgment SKM[S n] (.s (.mk n.succ))
+  | m n                       : valid_judgment SKM[M n] (.m (.mk n.succ))
+  | call lhs rhs              : lhs.max_universe > rhs.max_universe
+    → valid_judgment lhs (.call (.mk (Expr.m (.mk lhs.max_universe.succ)) lhs))
+    → valid_judgment rhs (.call (.mk (Expr.m (.mk rhs.max_universe.succ)) rhs))
+    → valid_judgment SKM[(lhs rhs)]
+      (.call (.mk
+        (.call (.mk
+          (Expr.m (.mk lhs.max_universe.succ))
+          lhs
+        ))
+        (.call (.mk
+          (Expr.m (.mk rhs.max_universe.succ))
+          rhs
+        ))
+      ))
+  | step_beta_eq e t₁ t₂           : valid_judgment e t₁ → is_eval_once t₁ t₂ → valid_judgment e t₂
+
+inductive valid_judgment_weak : Expr → Expr → Prop
+  | k n                       : valid_judgment_weak SKM[K n] (.k (.mk n.succ))
+  | s n                       : valid_judgment_weak SKM[S n] (.s (.mk n.succ))
+  | m n                       : valid_judgment_weak SKM[M n] (.m (.mk n.succ))
+  | call lhs rhs              : lhs.max_universe > rhs.max_universe
+    → valid_judgment_weak lhs (.call (.mk (Expr.m (.mk lhs.max_universe.succ)) lhs))
+    → valid_judgment_weak rhs (.call (.mk (Expr.m (.mk rhs.max_universe.succ)) rhs))
+    → valid_judgment_weak SKM[(lhs rhs)]
+      (.call (.mk
+        (.call (.mk
+          (Expr.m (.mk lhs.max_universe.succ))
+          lhs
+        ))
+        (.call (.mk
+          (Expr.m (.mk rhs.max_universe.succ))
+          rhs
+        ))
+      ))
+
+end
+
+inductive is_normal_n : ℕ → Expr → Expr → Prop
+  | stuck : (¬(∃ e', is_eval_once e e'))                 → is_normal_n 0 e e
+  | one   : is_eval_once e e                             → is_normal_n 1 e e
+  | succ  : is_eval_once e e' → is_normal_n n e' e_final → is_normal_n n.succ e e_final
+
+lemma m_stuck : is_normal_n 0 SKM[M n] SKM[M n] := by
+  apply is_normal_n.stuck
+  intro h
+  obtain ⟨e', h_eval⟩ := h
+  cases h_eval
+
+lemma k_stuck : is_normal_n 0 SKM[K n] SKM[K n] := by
+  apply is_normal_n.stuck
+  intro h
+  obtain ⟨e', h_eval⟩ := h
+  cases h_eval
+
+lemma s_stuck : is_normal_n 0 SKM[S n] SKM[S n] := by
+  apply is_normal_n.stuck
+  intro h
+  obtain ⟨e', h_eval⟩ := h
+  cases h_eval
+
