SkLean/Sn2.lean
@@ -1,0 +1,82 @@
+import SkLean.Ast2
+import Mathlib.Tactic
+
+inductive sn : Expr → Prop
+  | hard : (∀ e', is_eval_once e e' → sn e') → sn e
+
+lemma sn_call_k : sn SKM[(((K n) x) y)] → sn x := by
+  intro h_sn
+  match h_sn with
+    | .hard h_step =>
+      exact h_step x (by apply is_eval_once.k)
+
+lemma sn_call_s : sn SKM[((((S n) x) y) z)] → sn SKM[((x z) (y z))] := by
+  intro h_sn
+  match h_sn with
+    | .hard h_step =>
+      exact h_step SKM[((x z) (y z))] (by apply is_eval_once.s)
+
+lemma sn_m : sn SKM[(M n e)] → valid_judgment e t → sn t := by
+  intro h_sn h_t
+  match h_sn with
+    | .hard h_step =>
+      exact h_step t (by apply is_eval_once.m; exact h_t)
+
+lemma sn_preserved : sn e → is_eval_once e e' → sn e' := by
+  intro h_sn h_eval
+  cases e
+  cases h_eval
+  cases h_eval
+  cases h_eval
+  case call c =>
+    match h_sn with
+      | .hard h_step =>
+        exact h_step e' h_eval
+
+lemma sn_imp_n_steps_eval_normal (e : Expr) : sn e → ∃ n e', is_normal_n n e e' := by
+  intro h_sn
+  match h_eq : e with
+    | SKM[(M n₁)] =>
+      use 0
+      use SKM[(M n₁)]
+      apply m_stuck
+    | SKM[(K n)] =>
+      use 0
+      use SKM[(K n)]
+      apply k_stuck
+    | SKM[(S n)] =>
+      use 0
+      use SKM[(S n)]
+      apply s_stuck
+    | SKM[(((K n_k) x) y)] =>
+      match h_sn with
+        | .hard h =>
+          have h := h x (by apply is_eval_once.k)
+          have ⟨n, e_norm, h_norm_step⟩ := sn_imp_n_steps_eval_normal _ h
+          use n.succ
+          use e_norm
+          apply is_normal_n.succ
+          apply is_eval_once.k
+          exact h_norm_step
+    | SKM[((((S n) x) y) z)] =>
+      rw [← h_eq] at h_sn
+      induction h_sn
+      case hard e' h_step hh =>
+        have h_eval := is_eval_once.s x y z n
+        rw [h_eq] at h_step
+        rw [h_eq] at hh
+        have h_eval_sn := h_step _ h_eval
+        cases h_eval_sn
+        
+        sorry
+    | SKM[((M n) e)] =>
+      
+      sorry
+    | SKM[(lhs rhs)] =>
+      rw [← h_eq] at h_sn
+      induction h_sn
+      case hard e' h_step hh =>
+        simp_all
+        
+        sorry
+
