SkLean/SnProofHard.lean
@@ -1,0 +1,512 @@
+import Mathlib.Tactic
+import SkLean.DependentExamples
+
+theorem progress : valid_judgment e t → ∃ e', is_eval_once e e' := by
+  intro h_t
+  cases h_t
+  case k n =>
+    use SKM[K n]
+    apply is_eval_once.k_rfl
+  case s n =>
+    use SKM[S n]
+    apply is_eval_once.s_rfl
+  case m n =>
+    use SKM[M n]
+    apply is_eval_once.m_rfl
+  case call lhs rhs h_u h_t_lhs h_t_rhs =>
+    match h : SKM[(lhs rhs)] with
+      | SKM[(((K n) x) y)] =>
+        use x
+        apply is_eval_once.k
+      | SKM[(((S n x) y) z)] =>
+        use SKM[((x z) (y z))]
+        apply is_eval_once.s
+      | SKM[(M n e)] =>
+        use (.call (.mk (.m (.mk lhs.max_universe.succ)) lhs))
+        apply is_eval_once.m
+        simp_all
+        have h_t_lhs' := valid_judgment.step_beta_eq _ _ _ h_t_lhs (by
+          apply is_eval_once.m
+          apply valid_judgment.m
+        )
+        simp [Expr.max_universe] at *
+        apply valid_judgment.step_beta_eq
+        exact h_t_rhs
+        
+      | SKM[(lhs rhs)] =>
+        sorry
+      | _ => sorry
+  case step_beta_eq t' h_t' h_step =>
+    sorry
+
+namespace valid_judgment
+
+theorem beta_eq : valid_judgment e t₁ → beta_eq t₁ t₂ → valid_judgment e t₂ := by
+  intro h_t h_beq
+  cases h_beq
+  case rfl =>
+    exact h_t
+  case eval h =>
+    apply valid_judgment.step_beta_eq
+    exact h_t
+    exact h
+  case left lhs lhs' rhs h_eq' =>
+    cases h_t
+    case call lhs₁ rhs₁ h_u₁ h_t_lhs h_t_rhs =>
+      have h_t₀ := valid_judgment.call _ _ h_u₁ h_t_lhs h_t_rhs
+      
+    case step_beta_eq t₁ h_t₁ h_step =>
+      sorry
+  case right lhs rhs rhs' h_eq' =>
+    sorry
+  case trans e h_eq₁ h_eq₂ =>
+    sorry
+
+end valid_judgment
+
+lemma valid_judgment_imp_valid_universes_hard : valid_judgment e t → e.valid_universes := by
+  intro h_t
+  cases h_t
+  apply Expr.valid_universes.k
+  apply Expr.valid_universes.s
+  apply Expr.valid_universes.m
+  case call lhs rhs h_u h_t_lhs h_t_rhs =>
+    apply Expr.valid_universes.call
+    exact h_u
+    apply valid_judgment_imp_valid_universes_hard at h_t_lhs
+    exact h_t_lhs
+    apply valid_judgment_imp_valid_universes_hard at h_t_rhs
+    exact h_t_rhs
+  case beta_eq t' h_t_t' h_beta_eq_t' =>
+    cases h_t_t'
+    apply Expr.valid_universes.k
+    apply Expr.valid_universes.s
+    apply Expr.valid_universes.m
+    apply Expr.valid_universes.call
+    case call.a _ _ h_u _ _ =>
+      exact h_u
+    case call.a lhs rhs h_u h_t_lhs h_t_rhs =>
+      apply valid_judgment_imp_valid_universes_hard
+      exact h_t_lhs
+    case call.a lhs rhs h_u h_t_lhs h_t_rhs =>
+      apply valid_judgment_imp_valid_universes_hard
+      exact h_t_rhs
+    case beta_eq t_step h_t h_beq =>
+      cases h_beta_eq_t'
+      case rfl =>
+        cases h_beq
+        
+        sorry
+
+lemma valid_judgment_imp_m : ∀ n, valid_judgment e t → valid_judgment e SKM[((M n) e)] := by
+  intro n h
+  apply valid_judgment.beta_eq
+  exact h
+  apply beta_eq.symm
+  apply beta_eq.eval
+  apply is_eval_once.m
+  exact h
+
+lemma eval_preserves_judgment : ∀ e e' t, valid_judgment e t → is_eval_once e e' → valid_judgment e' t' → valid_judgment e' t := by
+  intro c e' t h_t h_eval h_t'
+  cases h_eval
+  case k y n =>
+    apply valid_judgment.beta_eq
+    apply valid_judgment_imp_m (e'.max_universe.succ)
+    exact h_t'
+    apply beta_eq.trans
+    apply beta_eq.eval
+    apply is_eval_once.m
+    exact h_t'
+    apply beta_eq.symm
+    apply beta_eq.trans
+    apply beta_eq.symm
+    apply beta_eq.eval
+    apply is_eval_once.m
+    use 0
+    exact h_t
+    apply beta_eq.trans
+    apply beta_eq.eval
+    apply is_eval_once.right
+    apply is_eval_once.k
+    apply beta_eq.eval
+    apply is_eval_once.m
+    exact h_t'
+  case s x y z n =>
+    apply valid_judgment.beta_eq
+    apply valid_judgment_imp_m (SKM[((x z) (y z))].max_universe.succ)
+    exact h_t'
+    apply beta_eq.trans
+    apply beta_eq.eval
+    apply is_eval_once.m
+    exact h_t'
+    apply beta_eq.symm
+    apply beta_eq.trans
+    apply beta_eq.symm
+    apply beta_eq.eval
+    apply is_eval_once.m
+    use 0
+    exact h_t
+    apply beta_eq.trans
+    apply beta_eq.eval
+    apply is_eval_once.right
+    apply is_eval_once.s
+    apply beta_eq.eval
+    apply is_eval_once.m
+    exact h_t'
+  case m e'' n h =>
+    apply valid_judgment.beta_eq
+    apply valid_judgment_imp_m (e''.max_universe.succ)
+    exact h_t'
+    apply beta_eq.trans
+    apply beta_eq.eval
+    apply is_eval_once.m
+    exact h_t'
+    apply beta_eq.symm
+    apply beta_eq.trans
+    apply beta_eq.symm
+    apply beta_eq.eval
+    apply is_eval_once.m
+    use 0
+    exact h_t
+    apply beta_eq.trans
+    apply beta_eq.eval
+    apply is_eval_once.right
+    apply is_eval_once.m
+    exact h
+    apply beta_eq.eval
+    apply is_eval_once.m
+    exact h_t'
+  case left lhs lhs' rhs h_eq =>
+    apply valid_judgment.beta_eq
+    apply valid_judgment_imp_m
+    use 0
+    exact h_t'
+    apply beta_eq.trans
+    apply beta_eq.right
+    apply beta_eq.left
+    apply beta_eq.symm
+    apply beta_eq.eval h_eq
+    apply beta_eq.eval
+    apply is_eval_once.m
+    exact h_t
+  case right rhs rhs' lhs h_eq =>
+    apply valid_judgment.beta_eq
+    apply valid_judgment_imp_m
+    use 0
+    exact h_t'
+    apply beta_eq.trans
+    apply beta_eq.right
+    apply beta_eq.right
+    apply beta_eq.symm
+    apply beta_eq.eval h_eq
+    apply beta_eq.eval
+    apply is_eval_once.m
+    exact h_t
+  case k_rfl =>
+    exact h_t
+  case s_rfl =>
+    exact h_t
+  case m_rfl =>
+    exact h_t
+
+lemma eval_preserves_judgment_hard' : ∀ e e' t, valid_judgment e t → is_eval_once e e' → valid_judgment e' t := by
+  intro e e' t h_t h_eval
+  cases h_t
+  case k n =>
+    cases h_eval
+    apply valid_judgment.k
+  case s =>
+    cases h_eval
+    apply valid_judgment.s
+  case m =>
+    cases h_eval
+    apply valid_judgment.m
+  case call lhs rhs h_u h_t_lhs h_t_rhs  =>
+    match h_e'_eq : e' with
+      | .m (.mk n) =>
+        apply valid_judgment.beta_eq
+        apply valid_judgment.m
+        apply beta_eq.symm
+        have h_eval_beq := beta_eq.eval h_eval
+        apply beta_eq.trans
+        apply beta_eq.left
+        apply beta_eq.eval
+        apply is_eval_once.m
+        exact h_t_lhs
+        apply beta_eq.symm
+        apply beta_eq.trans
+        apply beta_eq.symm
+        apply beta_eq.eval
+        apply is_eval_once.m
+        use n
+        apply valid_judgment.m
+        apply beta_eq.trans
+        apply beta_eq.right
+        exact (beta_eq.symm h_eval_beq)
+        apply beta_eq.trans
+        apply beta_eq.eval
+        apply is_eval_once.m
+        apply valid_judgment.call
+        exact h_u
+        exact h_t_lhs
+        exact h_t_rhs
+        apply beta_eq.rfl
+      | .k (.mk n) =>
+        apply valid_judgment.beta_eq
+        apply valid_judgment.k
+        apply beta_eq.symm
+        have h_eval_beq := beta_eq.eval h_eval
+        apply beta_eq.trans
+        apply beta_eq.left
+        apply beta_eq.eval
+        apply is_eval_once.m
+        exact h_t_lhs
+        apply beta_eq.symm
+        apply beta_eq.trans
+        apply beta_eq.symm
+        apply beta_eq.eval
+        apply is_eval_once.m
+        use n
+        apply valid_judgment.k
+        apply beta_eq.trans
+        apply beta_eq.right
+        exact (beta_eq.symm h_eval_beq)
+        apply beta_eq.trans
+        apply beta_eq.eval
+        apply is_eval_once.m
+        apply valid_judgment.call
+        exact h_u
+        exact h_t_lhs
+        exact h_t_rhs
+        apply beta_eq.rfl
+      | .s (.mk n) =>
+        apply valid_judgment.beta_eq
+        apply valid_judgment.s
+        apply beta_eq.symm
+        have h_eval_beq := beta_eq.eval h_eval
+        apply beta_eq.trans
+        apply beta_eq.left
+        apply beta_eq.eval
+        apply is_eval_once.m
+        exact h_t_lhs
+        apply beta_eq.symm
+        apply beta_eq.trans
+        apply beta_eq.symm
+        apply beta_eq.eval
+        apply is_eval_once.m
+        use n
+        apply valid_judgment.s
+        apply beta_eq.trans
+        apply beta_eq.right
+        exact (beta_eq.symm h_eval_beq)
+        apply beta_eq.trans
+        apply beta_eq.eval
+        apply is_eval_once.m
+        apply valid_judgment.call
+        exact h_u
+        exact h_t_lhs
+        exact h_t_rhs
+        apply beta_eq.rfl
+      | .call (.mk lhs' rhs') =>
+        have h_t_lhs' := eval_preserves_judgment_hard' lhs lhs' _ h_t_lhs
+        have h_t_rhs' := eval_preserves_judgment_hard' rhs rhs' _ h_t_rhs
+        cases h_eval
+        apply valid_judgment.beta_eq
+        apply valid_judgment.call
+        simp [Expr.max_universe] at *
+        
+        sorry
+
+lemma congr_m : valid_judgment a t
+  → valid_judgment b t
+  → beta_eq a b
+  → beta_eq (Expr.call (.mk (.m (.mk a.max_universe.succ)) a)) (.call (.mk (.m (.mk b.max_universe.succ)) b)) := by
+    intro h_t_lhs h_t_rhs h
+    simp [Expr.max_universe]
+    cases h_t_lhs
+    cases h_t_rhs
+    cases h
+    apply beta_eq.rfl
+    apply beta_eq.rfl
+    apply beta_eq.rfl
+    apply beta_eq.rfl
+    cases h
+    apply beta_eq.rfl
+    case k.beta_eq.eval rhs h₂ h₃ h₄ h₅ =>
+      simp [Expr.max_universe] at *
+      apply beta_eq.trans
+      apply beta_eq.eval
+      apply is_eval_once.m
+      apply valid_judgment.k
+      simp
+      apply beta_eq.symm
+      apply beta_eq.trans
+      apply beta_eq.eval
+      apply is_eval_once.m
+      exact h₃
+      exact h₄
+    case k.beta_eq.symm rhs h₂ h₃ h₄ h₅ =>
+      simp [Expr.max_universe] at *
+      apply beta_eq.trans
+      apply beta_eq.eval
+      apply is_eval_once.m
+      apply valid_judgment.k
+      simp
+      apply beta_eq.symm
+      apply beta_eq.trans
+      apply beta_eq.eval
+      apply is_eval_once.m
+      exact h₃
+      exact h₄
+    case k.beta_eq.trans rhs h_rhs h₂ h₃ h₄ h₅ =>
+      apply beta_eq.trans
+      apply beta_eq.right
+      exact h₄
+      apply beta_eq.trans
+      apply beta_eq.right
+      exact h₅
+      simp [Expr.max_universe]
+      apply beta_eq.trans
+      apply beta_eq.eval
+      apply is_eval_once.m
+      exact h_rhs
+      apply beta_eq.symm
+      apply beta_eq.trans
+      apply beta_eq.eval
+      apply is_eval_once.m
+      exact h_rhs
+      apply beta_eq.rfl
+    case s =>
+      apply beta_eq.trans
+      apply beta_eq.right
+      exact h
+      simp [Expr.max_universe]
+      apply beta_eq.symm
+      apply beta_eq.trans
+      apply beta_eq.eval
+      apply is_eval_once.m
+      exact h_t_rhs
+      simp
+      apply beta_eq.symm
+      apply beta_eq.trans
+      apply beta_eq.eval
+      apply is_eval_once.m
+      exact h_t_rhs
+      simp
+      exact beta_eq.rfl
+    case m =>
+      apply beta_eq.trans
+      apply beta_eq.right
+      exact h
+      simp [Expr.max_universe]
+      apply beta_eq.symm
+      apply beta_eq.trans
+      apply beta_eq.eval
+      apply is_eval_once.m
+      exact h_t_rhs
+      simp
+      apply beta_eq.symm
+      apply beta_eq.trans
+      apply beta_eq.eval
+      apply is_eval_once.m
+      exact h_t_rhs
+      simp
+      exact beta_eq.rfl
+    case call lhs rhs h_u h_t_lhs h_t_rhs =>
+      simp [Expr.max_universe] at *
+      apply beta_eq.trans
+      apply beta_eq.right
+      exact h
+      apply beta_eq.symm
+      apply beta_eq.trans
+      apply beta_eq.eval
+      apply is_eval_once.m
+      exact h_t_rhs
+      apply beta_eq.symm
+      apply beta_eq.trans
+      apply beta_eq.eval
+      apply is_eval_once.m
+      exact h_t_rhs
+      apply beta_eq.rfl
+    case beta_eq t' h_t' h_eq =>
+      have h_t_lhs'' := valid_judgment.beta_eq _ _ _ h_t' h_eq
+      have h_t_rhs'' := valid_judgment.beta_eq _ _ _ h_t_rhs (beta_eq.symm h_eq)
+      apply beta_eq.trans
+      apply beta_eq.right
+      exact h
+      apply beta_eq.trans
+      apply beta_eq.eval
+      apply is_eval_once.m
+      exact h_t_rhs''
+      apply beta_eq.symm
+      apply beta_eq.eval
+      apply is_eval_once.m
+      exact h_t_rhs''
+
+lemma valid_judgment_call_imp_judgment_lhs_rhs : valid_judgment SKM[(lhs rhs)] t → (∃ t_lhs, valid_judgment lhs t_lhs) ∧ (∃ t_rhs, valid_judgment rhs t_rhs) := by
+  intro h_t
+  cases h_t
+  case call h_t_lhs h_t_rhs h_u =>
+    constructor
+    use (.call (.mk (.m (.mk lhs.max_universe.succ)) lhs))
+    use (.call (.mk (.m (.mk rhs.max_universe.succ)) rhs))
+  case beta_eq t₂ h_t₂ h_t_beq =>
+    have h_t₃ := valid_judgment.beta_eq _ _ _ h_t₂ h_t_beq
+    constructor
+    cases h_t₂
+    case left.call =>
+      use (.call (.mk (.m (.mk lhs.max_universe.succ)) lhs))
+    case left.beta_eq =>
+      
+    sorry
+
+theorem all_well_typed_sn : ∀ e t, valid_judgment e t → sn e := by
+  intro e t h_t
+  cases h_t
+  case k =>
+    apply sn.trivial
+    apply is_eval_once.k_rfl
+  case s =>
+    apply sn.trivial
+    apply is_eval_once.s_rfl
+  case m =>
+    apply sn.trivial
+    apply is_eval_once.m_rfl
+  case call lhs rhs h_u h_t_lhs h_t_rhs =>
+    apply all_well_typed_sn_weak
+    
+  sorry
+
+theorem all_types_decideable : ∀ e t, valid_judgment e t → ∃ e, valid_judgment_weak e t := by
+  intro e t h_t
+  cases h_t
+  case k n =>
+    use SKM[K n]
+    apply valid_judgment_weak.k
+  case s n =>
+    use SKM[S n]
+    apply valid_judgment_weak.s
+  case m n =>
+    use SKM[M n]
+    apply valid_judgment_weak.m
+  case call lhs rhs h_u h_t_lhs h_t_rhs =>
+    apply all_types_decideable at h_t_lhs
+    apply all_types_decideable at h_t_rhs
+    have ⟨lhs', h_t_lhs'⟩ := h_t_lhs
+    have ⟨rhs', h_t_rhs'⟩ := h_t_rhs
+    use SKM[(lhs' rhs')]
+    cases h_t_lhs'
+  case beta_eq t' h_t' h_eq =>
+    cases e
+    case m =>
+      sorry
+    case k =>
+      sorry
+    case s =>
+      sorry
+    case call c =>
+      match c with
+        | .mk lhs rhs =>
+          
+          sorry
